Bdd/Reduce.lean
@@ -1,0 +1,118 @@
+import Bdd.Basic
+open List renaming Vector → Vec
+
+open Pointer
+open Bdd
+
+def OBdd.discover_helper : List (Fin m) → Vec (Node n m ) m → Vec (List (Fin m)) n → Vec (List (Fin m)) n
+  | [], _, I => I
+  | head :: tail, v, I => discover_helper tail v (I.set v[head].var (head :: I.get v[head].var))
+
+lemma OBdd.discover_helper_retains_found (O : OBdd n m) {I : Vec (List (Fin m)) n} : j ∈ I.get i → j ∈ (discover_helper l v I).get i := by
+  intro h
+  cases l with
+  | nil => assumption
+  | cons head tail =>
+    simp [discover_helper]
+    apply discover_helper_retains_found O
+    cases decEq v[head.1].var i with
+    | isFalse hf => rw [List.Vector.get_set_of_ne hf]; assumption
+    | isTrue  ht => subst ht; rw [List.Vector.get_set_same]; right; assumption
+
+lemma OBdd.discover_helper_spec (O : OBdd n m) {I : Vec (List (Fin m)) n} :
+    j ∈ l → j ∈ (discover_helper l v I).get v[j].var := by
+  intro h
+  cases h with
+  | head as =>
+    simp [discover_helper]
+    apply discover_helper_retains_found O
+    rw [List.Vector.get_set_same]
+    left
+  | tail b ih =>
+    simp [discover_helper]
+    apply discover_helper_spec O ih
+
+/-- Return a vector whose `v`th entry is a list of node indices with variable index `v`.
+
+This is a subroutine of `reduce`.  -/
+def OBdd.discover (O : OBdd n m) : Vec (List (Fin m)) n := discover_helper (collect O) O.1.heap (Vec.replicate n [])
+
+/-- `discover` is correct. -/
+theorem OBdd.discover_spec {O : OBdd n m} {j : Fin m} :
+    (Reachable O.1.heap O.1.root (node j)) → j ∈ (discover O).get O.1.heap[j].var :=
+  (discover_helper_spec O) ∘ collect_spec
+
+structure ReduceState (n) (m) where
+  subgraph : Vec (Node n m) m
+  ids : Vec (Pointer m) m
+  nextid : Fin m
+
+open ReduceState
+
+def ReduceState.initial {n m : Nat} : ReduceState n.succ m.succ := ⟨(Vec.replicate m.succ {var := 0, low := terminal false, high := terminal true}), (Vec.replicate m.succ (terminal false)), Fin.last m⟩
+
+def ReduceState.setId {n m} : Fin m → Pointer m → ReduceState n m → ReduceState n m :=
+  fun j id s ↦ ⟨s.subgraph, s.ids.set j id, s.nextid⟩
+
+def ReduceState.setSg {n m : Nat} : Node n.succ m.succ → ReduceState n.succ m.succ → ReduceState n.succ m.succ :=
+  fun N s ↦ ⟨s.subgraph.set (s.nextid + 1) N, s.ids, s.nextid + 1⟩
+
+def ReduceState.reduceId : ReduceState n m → Pointer m → Pointer m :=
+  fun s p ↦
+    match p with
+    | terminal b => terminal b
+    | node j     => s.ids[j]
+
+def OBdd.populate_queue (v : Vec (Node n m) m) (Q : List ((Pointer m × Pointer m) × Fin m)) (s : ReduceState n m) :
+    List (Fin m) → (List ((Pointer m × Pointer m) × Fin m) × ReduceState n m)
+  | [] => ⟨Q, s⟩
+  | u :: tail =>
+    let lid := s.reduceId v[u].low
+    let hid := s.reduceId v[u].high
+    if decide (lid = hid)
+    then populate_queue v Q (s.setId u lid) tail
+    else populate_queue v (⟨⟨lid, hid⟩, u⟩ :: Q) s tail
+
+def OBdd.reduce_process_queue {n m : Nat} (Q : List ((Pointer m.succ × Pointer m.succ) × Fin m.succ)) (curkey : Pointer m.succ × Pointer m.succ) (v : Vec (Node n.succ m.succ) m.succ) (s : ReduceState n.succ m.succ) : ReduceState n.succ m.succ :=
+  match Q with
+  | [] => s
+  | head :: tail =>
+    if head.1 = curkey
+    then
+      reduce_process_queue tail curkey v (s.setId head.2 (node s.nextid))
+    else
+      let s := s.setSg ⟨v[head.2].var, s.reduceId v[head.2].low, s.reduceId v[head.2].high⟩
+      let s := s.setId head.2 (node s.nextid)
+      reduce_process_queue tail head.1 v s
+
+def OBdd.reduce_step {n m : Nat} (vlist : Vec (List (Fin m.succ)) n.succ) (i : Fin n.succ) (v : Vec (Node n.succ m.succ) m.succ) (s : ReduceState n.succ m.succ) : ReduceState n.succ m.succ :=
+  let ⟨Q, s⟩ := populate_queue v [] s vlist[i]
+  reduce_process_queue (List.mergeSort Q) ⟨node 0, node 0⟩ v s
+
+def OBdd.reduce_loop {n m : Nat} (vlist : Vec (List (Fin m.succ)) n.succ) (v : Vec (Node n.succ m.succ) m.succ) (r : Fin m.succ) (i : Fin n.succ) (s : ReduceState n.succ m.succ) : Bdd n.succ m.succ :=
+  let s := reduce_step vlist i v s
+  match h : i.1 - v[r].var.1 with
+  | Nat.zero    => {heap := s.subgraph, root := s.reduceId (node r)}
+  | Nat.succ j  => reduce_loop vlist v r ⟨(j + v[r].var.1), by omega⟩ s
+termination_by i.1 - v[r].var.1
+decreasing_by simp_all
+
+def OBdd.reduce {n m : Nat} (O : OBdd n.succ m.succ) : Bdd n.succ m.succ :=
+  match O.1.root with
+  | terminal _ => O.1 -- Terminals are already reduced.
+  | node r => reduce_loop (discover O) O.1.heap r n initial
+
+def example_not_reduced_bdd : OBdd 3 5 :=
+  ⟨ { heap := ⟨[{var := 0, low := node 1, high := node 2},
+                 {var := 1, low := terminal false, high := node 4},
+                 {var := 1, low := node 3, high := terminal true},
+                 {var := 2, low := terminal false, high := terminal true},
+                 {var := 2, low := terminal false, high := terminal true}], rfl⟩
+      root := node 0 },
+    by apply Ordered_of_Proper; decide⟩
+
+#eval example_not_reduced_bdd.reduce
+
+private lemma ordered_after_reduce : example_not_reduced_bdd.reduce.Ordered := by apply Ordered_of_Proper; decide (config := {kernel := true})
+
+example : OBdd.Reduced ⟨example_not_reduced_bdd.reduce, ordered_after_reduce⟩ := by decide (config := {kernel := true})
